code/hash/Hacl.Hash.Core.Blake2.fsti
@@ -7,8 +7,12 @@ noextract inline_for_extraction
 val alloca_blake2s: alloca_st Blake2S
 val init_blake2s: init_st Blake2S
 val update_blake2s: update_st Blake2S
+val pad_blake2s: pad_st Blake2S
+val finish_blake2s: finish_st Blake2S
 
 noextract inline_for_extraction
 val alloca_blake2b: alloca_st Blake2B
 val init_blake2b: init_st Blake2B
 val update_blake2b: update_st Blake2B
+val pad_blake2b: pad_st Blake2B
+val finish_blake2b: finish_st Blake2B
